src/extraction.v
@@ -15,17 +15,13 @@ From marble Require Import int loop.
 Extraction Inline iter_down iter_up xiter_up uxiter_up.
 Extraction Inline Ni.
 Extraction Inline iter_down_unrolled iter_up_unrolled.
-Extraction Inline iter_down_N iter_upN.
+Extraction Inline iter_down_N iter_up_N.
 
 (* Recursive Extraction iter_down iter_up xiter_up uxiter_up. *)
 
 From Stdlib Require ExtrOCamlPArray.
 From marble Require Import array.
 Extraction Inline to_list.
-Extraction Inline Ni.
-Extraction Inline simple_blit blitN.
-Extraction Inline simple_blit'_up simple_blit'_down.
-Extraction Inline blit'_up blit'_down.
 
 (* Recursive Extraction of_list blit blit' copy find_index equal. *)
 
